src/Parsers/Reachable/ParenBalanced/OfParse.v
@@ -1,0 +1,194 @@
+(** * Every parse tree has a corresponding minimal parse tree *)
+Require Import Coq.Program.Basics.
+Require Import Coq.Strings.String Coq.Lists.List Coq.Setoids.Setoid Coq.Classes.RelationClasses Coq.Classes.Morphisms.
+Require Import Fiat.Parsers.ContextFreeGrammar.
+Require Import Fiat.Parsers.ContextFreeGrammarProperties.
+Require Import Fiat.Parsers.StringLike.ForallChars.
+Require Import Fiat.Parsers.Reachable.ParenBalanced.Core.
+Require Import Fiat.Parsers.Reachable.ParenBalanced.MinimalOfCore.
+Require Import Fiat.Parsers.BaseTypes.
+Require Import Fiat.Parsers.BaseTypesLemmas.
+Require Import Fiat.Common.
+
+Set Implicit Arguments.
+Local Open Scope string_like_scope.
+
+Section cfg.
+  Context {Char} {HSL : StringLike Char} {HSLP : StringLikeProperties Char} {G : grammar Char}.
+  Context {predata : parser_computational_predataT}
+          {rdata' : @parser_removal_dataT' predata}.
+
+  Definition parse_empty_pb_parse_of_item'
+             (parse_empty_pb_parse_of_productions
+              : forall valid0 pats
+                       (str : String) (Hlen : length str = 0) (p : parse_of G str pats)
+                       (Hforall : Forall_parse_of (fun _ nt' => is_valid_nonterminal valid0 nt') p),
+                  pb_productions G valid0 pats)
+             {valid0 it}
+             (str : String) (Hlen : length str = 0) (p : parse_of_item G str it)
+             (Hforall : Forall_parse_of_item (fun _ nt' => is_valid_nonterminal valid0 nt') p)
+  : pb_item G valid0 it.
+  Proof.
+    destruct p as [ | nt p ].
+    { exfalso.
+      erewrite length_singleton in Hlen by eassumption; omega. }
+    { specialize (parse_empty_pb_parse_of_productions valid0 (G nt) str Hlen p (snd Hforall)).
+      constructor; simpl in *; [ exact (fst Hforall) | assumption ]. }
+  Defined.
+
+  Fixpoint parse_empty_pb_parse_of_productions
+             {valid0 pats}
+             (str : String) (Hlen : length str = 0) (p : parse_of G str pats)
+             (Hforall : Forall_parse_of (fun _ nt' => is_valid_nonterminal valid0 nt') p)
+             {struct p}
+  : pb_productions G valid0 pats
+  with parse_empty_pb_parse_of_production
+         {valid0 pat}
+         (str : String) (Hlen : length str = 0) (p : parse_of_production G str pat)
+         (Hforall : Forall_parse_of_production (fun _ nt' => is_valid_nonterminal valid0 nt') p)
+         {struct p}
+       : pb_production G valid0 pat.
+  Proof.
+    { destruct p as [ ?? p | ?? p ]; simpl in *.
+      { pose proof (parse_empty_pb_parse_of_production valid0 _ _ Hlen p Hforall).
+        left; assumption. }
+      { pose proof (parse_empty_pb_parse_of_productions valid0 _ _ Hlen p Hforall).
+        right; assumption. } }
+    { destruct p as [ | ?? p ]; simpl in *.
+      { constructor. }
+      { constructor.
+        { apply (fun k => @parse_empty_pb_parse_of_item' parse_empty_pb_parse_of_productions valid0 _ _ k _ (fst Hforall)).
+          rewrite take_length, Hlen, Min.min_0_r; reflexivity. }
+        { apply (fun k => @parse_empty_pb_parse_of_production valid0 _ _ k _ (snd Hforall)).
+          rewrite drop_length, Hlen; reflexivity. } } }
+  Defined.
+
+  Definition parse_empty_pb_parse_of_item
+             {valid0 it}
+             (str : String) (Hlen : length str = 0) (p : parse_of_item G str it)
+             (Hforall : Forall_parse_of_item (fun _ nt' => is_valid_nonterminal valid0 nt') p)
+  : pb_item G valid0 it
+    := @parse_empty_pb_parse_of_item' (@parse_empty_pb_parse_of_productions) valid0 it str Hlen p Hforall.
+
+  Definition parse_empty_minimal_pb_parse_of_item
+             {valid0 it}
+             (str : String) (Hlen : length str = 0) (p : parse_of_item G str it)
+             (Hforall : Forall_parse_of_item (fun _ nt' => is_valid_nonterminal valid0 nt') p)
+  : minimal_pb_item (G := G) valid0 it.
+  Proof.
+    eapply minimal_pb_item__of__pb_item.
+    eapply parse_empty_pb_parse_of_item; eassumption.
+  Qed.
+
+  Definition parse_empty_minimal_pb_parse_of_production
+             {valid0 pat}
+             (str : String) (Hlen : length str = 0) (p : parse_of_production G str pat)
+             (Hforall : Forall_parse_of_production (fun _ nt' => is_valid_nonterminal valid0 nt') p)
+  : minimal_pb_production (G := G) valid0 pat.
+  Proof.
+    eapply minimal_pb_production__of__pb_production.
+    eapply parse_empty_pb_parse_of_production; eassumption.
+  Qed.
+
+  Definition parse_empty_minimal_pb_parse_of_productions
+             {valid0 pats}
+             (str : String) (Hlen : length str = 0) (p : parse_of G str pats)
+             (Hforall : Forall_parse_of (fun _ nt' => is_valid_nonterminal valid0 nt') p)
+  : minimal_pb_productions (G := G) valid0 pats.
+  Proof.
+    eapply minimal_pb_productions__of__pb_productions.
+    eapply parse_empty_pb_parse_of_productions; eassumption.
+  Qed.
+
+  Definition parse_empty_from_pb_parse_of_item'
+             (parse_empty_from_pb_parse_of_productions
+              : forall valid0 pats
+                       (str : String) (Hlen : length str = 0),
+                  pb_productions G valid0 pats
+                  -> { p : parse_of G str pats
+                           & Forall_parse_of (fun _ nt' => is_valid_nonterminal valid0 nt') p })
+             {valid0 it}
+             (str : String) (Hlen : length str = 0)
+             (p : pb_item G valid0 it)
+  : { p : parse_of_item G str it
+          & Forall_parse_of_item (fun _ nt' => is_valid_nonterminal valid0 nt') p }.
+  Proof.
+    destruct p as [ nt H p ].
+    eapply parse_empty_from_pb_parse_of_productions in p; [ | eassumption.. ].
+    exists (ParseNonTerminal _ (projT1 p)).
+    exact (H, projT2 p).
+  Defined.
+
+  Fixpoint parse_empty_from_pb_parse_of_productions
+             {valid0 pats}
+             (str : String) (Hlen : length str = 0)
+             (p : pb_productions G valid0 pats)
+             {struct p}
+  : { p : parse_of G str pats
+          & Forall_parse_of (fun _ nt' => is_valid_nonterminal valid0 nt') p }
+  with parse_empty_from_pb_parse_of_production
+         {valid0 pat}
+         (str : String) (Hlen : length str = 0)
+         (p: pb_production G valid0 pat)
+         {struct p}
+       : { p : parse_of_production G str pat
+               & Forall_parse_of_production (fun _ nt' => is_valid_nonterminal valid0 nt') p }.
+  Proof.
+    { destruct p as [ ?? p | ?? p ]; simpl in *.
+      { pose proof (parse_empty_from_pb_parse_of_production valid0 _ _ Hlen p) as p'.
+        eexists (ParseHead _ (projT1 p')).
+        exact (projT2 p'). }
+      { pose proof (parse_empty_from_pb_parse_of_productions valid0 _ _ Hlen p) as p'.
+        eexists (ParseTail _ (projT1 p')).
+        exact (projT2 p'). } }
+    { destruct p as [ | ?? p0 p1 ]; simpl in *.
+      { exists (ParseProductionNil G _ Hlen). constructor. }
+      { eapply (@parse_empty_from_pb_parse_of_item' parse_empty_from_pb_parse_of_productions) in p0.
+        eapply (@parse_empty_from_pb_parse_of_production) in p1.
+        { eexists (ParseProductionCons _ 0 (projT1 p0) (projT1 p1)).
+          exact (projT2 p0, projT2 p1). }
+        { rewrite ?take_length, ?drop_length, Hlen; reflexivity. }
+        { rewrite ?take_length, ?drop_length, Hlen, Min.min_0_r; reflexivity. } } }
+  Defined.
+
+  Definition parse_empty_from_pb_parse_of_item
+             {valid0 it}
+             (str : String) (Hlen : length str = 0)
+             (p : pb_item G valid0 it)
+  : { p : parse_of_item G str it
+          & Forall_parse_of_item (fun _ nt' => is_valid_nonterminal valid0 nt') p }
+    := @parse_empty_from_pb_parse_of_item' (@parse_empty_from_pb_parse_of_productions) valid0 it str Hlen p.
+
+  Definition parse_empty_from_minimal_pb_parse_of_item
+             {valid0 it}
+             (str : String) (Hlen : length str = 0)
+             (p : minimal_pb_item (G := G) valid0 it)
+  : { p : parse_of_item G str it
+          & Forall_parse_of_item (fun _ nt' => is_valid_nonterminal valid0 nt') p }.
+  Proof.
+    eapply parse_empty_from_pb_parse_of_item; trivial.
+    eapply pb_item__of__minimal_pb_item; try eassumption; reflexivity.
+  Qed.
+
+  Definition parse_empty_from_minimal_pb_parse_of_production
+             {valid0 pat}
+             (str : String) (Hlen : length str = 0)
+             (p : minimal_pb_production (G := G) valid0 pat)
+  : { p : parse_of_production G str pat
+          & Forall_parse_of_production (fun _ nt' => is_valid_nonterminal valid0 nt') p }.
+  Proof.
+    eapply parse_empty_from_pb_parse_of_production; trivial.
+    eapply pb_production__of__minimal_pb_production; try eassumption; reflexivity.
+  Qed.
+
+  Definition parse_empty_from_minimal_pb_parse_of_productions
+             {valid0 pats}
+             (str : String) (Hlen : length str = 0)
+             (p : minimal_pb_productions (G := G) valid0 pats)
+  : { p : parse_of G str pats
+          & Forall_parse_of (fun _ nt' => is_valid_nonterminal valid0 nt') p }.
+  Proof.
+    eapply parse_empty_from_pb_parse_of_productions; trivial.
+    eapply pb_productions__of__minimal_pb_productions; try eassumption; reflexivity.
+  Qed.
+End cfg.
