src/Parsers/Reachable/ParenBalanced/WellFounded.v
@@ -5,7 +5,7 @@ Require Import Fiat.Parsers.BaseTypes.
 
 Section rel.
   Context {Char} {HSL : StringLike Char} {predata : parser_computational_predataT}
-          {pdata : paren_balanced_dataT Char}
+          {pdata : paren_balanced_hiding_dataT Char}
           {G : grammar Char}.
 
   Section size.
